Prove spec for retrying readonly syscalls
Turns out it's unsafe to run a possibly modifying system call under
readonly_syscall: it might make a modification that can't be committed
in readonly_syscall if no I/O is required, violating its specification
(although the return value will reflect what it would have returned,
which is fairly useless for the file system).

As such, retry_syscall is now retry_readonly_syscall and is still
required to commit readonly system calls that update the memstate, while
known modifying system calls (that is, those that want to update the
directory tree abstraction) must use write_syscall directly.

src/ConcurrentFS.v
@@ -1,3 +1,5 @@
+Require Import FunctionalExtensionality.
+
 Require Import CCL.
 Require Import Hashmap.
 
@@ -105,11 +107,13 @@ Section ConcurrentFS.
                       end)
              end).
 
-  Definition retry_syscall T (p: OptimisticProg T) (update: T -> dirtree -> dirtree) :=
+  (* to finish up read-only syscalls if they want to update the memory, we have
+  to run them under write_syscall *)
+  Definition retry_readonly_syscall T (p: OptimisticProg T) :=
     r <- readonly_syscall p;
       match r with
       | Done v => Ret (Done v)
-      | TryAgain => write_syscall p update
+      | TryAgain => write_syscall p (fun _ tree => tree)
       | SyscallFailed => Ret SyscallFailed
       end.
 
@@ -410,7 +414,7 @@ Section ConcurrentFS.
                                         Sigma.init_disk sigma' = Sigma.disk sigma'
                              | TryAgain => tree'' = tree' /\
                                           Sigma.init_disk sigma' = Sigma.disk sigma'
-                             | SyscallFailed => True
+                             | SyscallFailed => tree'' = tree'
                              end |})
                  (write_syscall p update).
   Proof using Type.
@@ -547,7 +551,7 @@ Section ConcurrentFS.
                                         tree'' = fs_dirup (fsspec a) v tree' /\
                                         Sigma.init_disk sigma' = Sigma.disk sigma'
                              | TryAgain => False
-                             | SyscallFailed => True
+                             | SyscallFailed => tree'' = tree'
                              end |})
                  (write_syscall p update).
   Proof using Type.
@@ -563,84 +567,135 @@ Section ConcurrentFS.
     destruct r; (intuition eauto); discriminate.
   Qed.
 
+  Theorem retry_readonly_syscall_ok : forall T (p: OptimisticProg T) A
+                               (fsspec: FsSpec A T) tid,
+      (forall mscs c l, cprog_spec G tid
+                              (fs_spec P fsspec tid mscs l c)
+                              (p mscs l c)) ->
+      cprog_spec G tid
+                 (fun '(tree, homedirs, a) sigma =>
+                    {| precondition :=
+                         fs_inv(P, sigma, tree, homedirs) /\
+                         local_l tid (Sigma.l sigma) = Unacquired /\
+                         fs_pre (fsspec a) tree /\
+                         (forall r tree, fs_dirup (fsspec a) r tree = tree) /\
+                         precondition_stable fsspec homedirs tid;
+                       postcondition :=
+                         fun sigma' r =>
+                           exists tree',
+                             fs_inv(P, sigma', tree', homedirs) /\
+                             homedir_rely tid homedirs tree tree' /\
+                             local_l tid (Sigma.l sigma') = Unacquired /\
+                             match r with
+                             | Done v => fs_post (fsspec a) v
+                             | TryAgain => False
+                             | SyscallFailed => True
+                             end |})
+                 (retry_readonly_syscall p).
+  Proof.
+    unfold retry_readonly_syscall; intros.
+
+    unfold cprog_spec; intros.
+    eapply cprog_ok_weaken;
+      [ monad_simpl; eapply readonly_syscall_ok; eauto | ];
+      simplify; finish.
+
+    destruct r.
+    - step; finish.
+    - eapply cprog_ok_weaken;
+      [ monad_simpl; eapply write_syscall_ok; eauto | ];
+      simplify; finish.
+      extensionality r.
+      extensionality tree0.
+      eauto.
+
+      step; finish.
+      destruct r; intuition subst.
+      match goal with
+      | [ H: context[fs_dirup (fsspec _)] |- _ ] =>
+        rewrite H
+      end.
+      etransitivity; eauto.
+      etransitivity; eauto.
+
+      destruct_goal_matches; intuition eauto.
+    - step; finish.
+  Qed.
+
   (* translate all system calls for extraction *)
 
   Definition file_get_attr inum :=
-    retry_syscall (fun mscs => file_get_attr (fsxp P) inum mscs)
-                  (fun _ tree => tree).
+    retry_readonly_syscall (fun mscs => file_get_attr (fsxp P) inum mscs).
 
   Definition lookup dnum names :=
-    retry_syscall (fun mscs => lookup (fsxp P) dnum names mscs)
-                  (fun _ tree => tree).
+    retry_readonly_syscall (fun mscs => lookup (fsxp P) dnum names mscs).
 
   Definition read_fblock inum off :=
-    retry_syscall (fun mscs => OptFS.read_fblock (fsxp P) inum off mscs)
-                  (fun _ tree => tree).
+    retry_readonly_syscall (fun mscs => OptFS.read_fblock (fsxp P) inum off mscs).
+
+  (* TODO: add real directory updates to these modifying system calls *)
 
   Definition file_set_attr inum attr :=
-    retry_syscall (fun mscs => OptFS.file_set_attr (fsxp P) inum attr mscs)
+    write_syscall (fun mscs => OptFS.file_set_attr (fsxp P) inum attr mscs)
                   (fun _ tree => tree).
 
   Definition file_truncate inum sz :=
-    retry_syscall (fun mscs => OptFS.file_truncate (fsxp P) inum sz mscs)
+    write_syscall (fun mscs => OptFS.file_truncate (fsxp P) inum sz mscs)
                   (fun _ tree => tree).
 
   Definition update_fblock_d inum off b :=
-    retry_syscall (fun mscs => OptFS.update_fblock_d (fsxp P) inum off b mscs)
+    write_syscall (fun mscs => OptFS.update_fblock_d (fsxp P) inum off b mscs)
                   (fun _ tree => tree).
 
   Definition create dnum name :=
-    retry_syscall (fun mscs => OptFS.create (fsxp P) dnum name mscs)
+    write_syscall (fun mscs => OptFS.create (fsxp P) dnum name mscs)
                   (fun _ tree => tree).
 
   Definition rename dnum srcpath srcname dstpath dstname :=
-    retry_syscall (fun mscs => OptFS.rename (fsxp P) dnum srcpath srcname dstpath dstname mscs)
+    write_syscall (fun mscs => OptFS.rename (fsxp P) dnum srcpath srcname dstpath dstname mscs)
                   (fun _ tree => tree).
 
   Definition delete dnum name :=
-    retry_syscall (fun mscs => OptFS.delete (fsxp P) dnum name mscs)
+    write_syscall (fun mscs => OptFS.delete (fsxp P) dnum name mscs)
                   (fun _ tree => tree).
 
   (* wrap unverified syscalls *)
 
   Definition statfs :=
-    retry_syscall (fun mscs => OptFS.statfs (fsxp P) mscs)
-                  (fun _ tree => tree).
+    retry_readonly_syscall (fun mscs => OptFS.statfs (fsxp P) mscs).
 
   Definition mkdir dnum name :=
-    retry_syscall (fun mscs => OptFS.mkdir (fsxp P) dnum name mscs)
+    write_syscall (fun mscs => OptFS.mkdir (fsxp P) dnum name mscs)
                   (fun _ tree => tree).
 
   Definition file_get_sz inum :=
-    retry_syscall (fun mscs => OptFS.file_get_sz (fsxp P) inum mscs)
-                  (fun _ tree => tree).
+    retry_readonly_syscall (fun mscs => OptFS.file_get_sz (fsxp P) inum mscs).
 
   Definition file_set_sz inum sz :=
-    retry_syscall (fun mscs => OptFS.file_set_sz (fsxp P) inum sz mscs)
+    write_syscall (fun mscs => OptFS.file_set_sz (fsxp P) inum sz mscs)
                   (fun _ tree => tree).
 
   Definition readdir dnum :=
-    retry_syscall (fun mscs => OptFS.readdir (fsxp P) dnum mscs)
-                  (fun _ tree => tree).
+    retry_readonly_syscall (fun mscs => OptFS.readdir (fsxp P) dnum mscs).
 
   Definition tree_sync :=
-    retry_syscall (fun mscs => OptFS.tree_sync (fsxp P) mscs)
+    write_syscall (fun mscs => OptFS.tree_sync (fsxp P) mscs)
                   (fun _ tree => tree).
 
   Definition file_sync inum :=
-    retry_syscall (fun mscs => OptFS.file_sync (fsxp P) inum mscs)
+    write_syscall (fun mscs => OptFS.file_sync (fsxp P) inum mscs)
                   (fun _ tree => tree).
 
   Definition update_fblock inum off b :=
-    retry_syscall (fun mscs => OptFS.update_fblock (fsxp P) inum off b mscs)
+    write_syscall (fun mscs => OptFS.update_fblock (fsxp P) inum off b mscs)
                   (fun _ tree => tree).
 
   Definition mksock dnum name :=
-    retry_syscall (fun mscs => OptFS.mksock (fsxp P) dnum name mscs)
+    write_syscall (fun mscs => OptFS.mksock (fsxp P) dnum name mscs)
                   (fun _ tree => tree).
 
   Definition umount :=
-    retry_syscall (fun mscs => OptFS.umount (fsxp P) mscs)
+    write_syscall (fun mscs => OptFS.umount (fsxp P) mscs)
                   (fun _ tree => tree).
 
 End ConcurrentFS.
